# 1685. Sum of Absolute Differences in a Sorted Array

*   You are given an integer array `nums` sorted in **non-decreasing** order.

    Build and return _an integer array_ `result` _with the same length as_ `nums` _such that_ `result[i]` _is equal to the **summation of absolute differences** between_ `nums[i]` _and all the other elements in the array._

    In other words, `result[i]` is equal to `sum(|nums[i]-nums[j]|)` where `0 <= j < nums.length` and `j != i` (**0-indexed**).
* **Constraints:**
  * `2 <= nums.length <= 105`
  * `1 <= nums[i] <= nums[i + 1] <= 104`

**Example 1:**

```java
Input: nums = [2,3,5]
Output: [4,3,5]
Explanation: Assuming the arrays are 0-indexed, then
result[0] = |2-2| + |2-3| + |2-5| = 0 + 1 + 3 = 4,
result[1] = |3-2| + |3-3| + |3-5| = 1 + 0 + 2 = 3,
result[2] = |5-2| + |5-3| + |5-5| = 3 + 2 + 0 = 5.
```

**Example 2:**

```java
Input: nums = [1,4,6,8,10]
Output: [24,15,13,15,21]
```

{% hint style="info" %}
simple brute force(time limit exceeded)

try to simplify it.
{% endhint %}

```java
public int[] getSumAbsoluteDifferences(int[] nums) {
    int[] result = new int[nums.length];
    for(int i = 0; i < nums.length; i++){
        int sum = 0;
        for(int j = 0; j < nums.length; j++){
            sum += Math.abs(nums[i] - nums[j]);
        }
        result[i] = sum;
    }
    return result;
}
```

{% hint style="info" %}
We can use **prefix sum and postfix sum** to solve this problem. The trick part is how to find the formula.

Look at the veido about how to generalize the formula

[https://www.youtube.com/watch?v=WYe644djV30](https://www.youtube.com/watch?v=WYe644djV30)

nums: \[1, 4, 6, 8, 10]

prefix sum from 0 to n - 1: \[0, 1, 5, 11, 19]

postfix sum from right(n - 2) to left(0): \[28, 24, 18, 10, 0]
{% endhint %}

```java
public int[] getSumAbsoluteDifferences(int[] nums) {
    int len = nums.length;
    int[] preSums = new int[len];
    for(int i = 1; i < len; i++)
        preSums[i] = preSums[i - 1] + nums[i - 1];
    
    int[] postSums = new int[len];
    for(int i = len - 2; i >= 0; i--)
        postSums[i] = postSums[i + 1] + nums[i + 1];
    
    int[] result = new int[len];
    for(int i = 0; i < len; i++)
        result[i] = i * nums[i] - (len - i - 1) * nums[i] - preSums[i] + postSums[i];
    return result;
}
```
